chore: fork with buffers and multiplle lowerings for different placements

SSA/Projects/CIRCT/HandshakeToHW/fork.lean
@@ -6,45 +6,30 @@ import SSA.Projects.CIRCT.Register.Lemmas
 namespace HandshakeStream
 
 /-!
+  # Fork
+
+  `fork` replicates the content of an input stream and dispatches it to two channels.
+  At the handshake level, `fork` operates on the `Stream' (Option α)` type (i.e., `Stream`).
+
+  We insert buffers in the handshake program and lower it to rtl level, considering all the
+  buffer configurations CIRCT inserts.
+
+  The hardware (lowered) module is a function over the `Stream'` type,
+  which does not contain `Option` values, because at this level
+  of abstractions the content of streams has been concretized.
+
+  See: https://github.com/opencompl/DC-semantics-simulation-evaluation/commit/bef3960435bc638477cb7ece87879c3ba2703473
+
+-/
+
+/--
   Handshake program:
 
     handshake.func @test_fork(%arg0: none, %arg1: none, ...) -> (none, none, none) {
       %0:2 = fork [2] %arg0 : none
       return %0#0, %0#1, %arg1 : none, none, none
     }
-
-  Lowered program (https://github.com/opencompl/DC-semantics-simulation-evaluation/commit/28ef888954a8726d4858bed925ad067729207655)
-
-  module {
-    hw.module @test_fork(in %arg0 : !esi.channel<i0>, in %arg1 : !esi.channel<i0>, in %clk : !seq.clock {dc.clock}, in %rst : i1 {dc.reset}, out out0 : !esi.channel<i0>, out out1 : !esi.channel<i0>, out out2 : !esi.channel<i0>) {
-      %rawOutput, %valid = esi.unwrap.vr %arg0, %12 : i0
-      %c0_i0 = hw.constant 0 : i0
-      %chanOutput, %ready = esi.wrap.vr %c0_i0, %3 : i0
-      %c0_i0_0 = hw.constant 0 : i0
-      %chanOutput_1, %ready_2 = esi.wrap.vr %c0_i0_0, %9 : i0
-      %false = hw.constant false
-      %true = hw.constant true
-      %0 = comb.xor %12, %true : i1
-      %1 = comb.and %5, %0 : i1
-      %emitted_0 = seq.compreg sym @emitted_0 %1, %clk reset %rst, %false : i1
-      %2 = comb.xor %emitted_0, %true : i1
-      %3 = comb.and %2, %valid : i1
-      %4 = comb.and %ready, %3 : i1
-      %5 = comb.or %4, %emitted_0 {sv.namehint = "done0"} : i1
-      %6 = comb.xor %12, %true : i1
-      %7 = comb.and %11, %6 : i1
-      %emitted_1 = seq.compreg sym @emitted_1 %7, %clk reset %rst, %false : i1
-      %8 = comb.xor %emitted_1, %true : i1
-      %9 = comb.and %8, %valid : i1
-      %10 = comb.and %ready_2, %9 : i1
-      %11 = comb.or %10, %emitted_1 {sv.namehint = "done1"} : i1
-      %12 = comb.and %5, %11 {sv.namehint = "allDone"} : i1
-      hw.output %chanOutput, %chanOutput_1, %arg1 : !esi.channel<i0>, !esi.channel<i0>, !esi.channel<i0>
-    }
-  }
 -/
-
-
 def fork_handshake (arg : Stream (BitVec 1)) :=
   corec_prod (β := Stream (BitVec 1)) arg
     fun x => Id.run <| do
@@ -53,58 +38,155 @@ def fork_handshake (arg : Stream (BitVec 1)) :=
       (x0, x0, x')
 
 /--
-  `fork` replicates the content of an input stream and dispatches it to two channels.
+  The first configuration of the rtl-lowered program
 
-  The hardware (lowered) module is a function over the `Stream'` type,
-  which does not contain `Option` values, because at this level
-  of abstractions the content of streams has been concretized.
+  hw.module @handshake_fork_1ins_2outs_ctrl(in %in0 : i0, in %in0_valid : i1, in %clock : !seq.clock, in %reset : i1, in %out0_ready : i1, in %out1_ready : i1, out in0_ready : i1, out out0 : i0, out out0_valid : i1, out out1 : i0, out out1_valid : i1) {
+    %true = hw.constant true
+    %false = hw.constant false
+    %0 = comb.xor %12, %true : i1
+    %1 = comb.and %5, %0 : i1
+    %emitted_0 = seq.compreg sym @emitted_0 %1, %clock reset %reset, %false : i1
+    %2 = comb.xor %emitted_0, %true : i1
+    %3 = comb.and %2, %in0_valid : i1
+    %4 = comb.and %out0_ready, %3 : i1
+    %5 = comb.or %4, %emitted_0 {sv.namehint = "done0"} : i1
+    %6 = comb.xor %12, %true : i1
+    %7 = comb.and %11, %6 : i1
+    %emitted_1 = seq.compreg sym @emitted_1 %7, %clock reset %reset, %false : i1
+    %8 = comb.xor %emitted_1, %true : i1
+    %9 = comb.and %8, %in0_valid : i1
+    %10 = comb.and %out1_ready, %9 : i1
+    %11 = comb.or %10, %emitted_1 {sv.namehint = "done1"} : i1
+    %12 = comb.and %5, %11 {sv.namehint = "allDone"} : i1
+    hw.output %12, %in0, %3, %in0, %9 : i1, i0, i1, i0, i1
+  }
 -/
-def fork_seq
-      (arg_0 : Stream' (BitVec 1))
-      (arg_0_valid : Stream' (BitVec 1))
-      (arg_1 : Stream' (BitVec 1))
-      (arg_1_valid : Stream' (BitVec 1))
+def handshake_fork_1ins_2outs_ctrl
+      (in0 : Stream' (BitVec 1))
+      (in0_valid : Stream' (BitVec 1))
       (out0_ready : Stream' (BitVec 1))
       (out1_ready : Stream' (BitVec 1))
-      (out2_ready : Stream' (BitVec 1))
-  : Vector (Stream' (BitVec 1)) 8 :=
+  : Vector (Stream' (BitVec 1)) 5 :=
     let vec_streams := streams_to_vec'
-                        (#v[arg_0, arg_0_valid, arg_1, arg_1_valid, out0_ready, out1_ready, out2_ready])
+                        (#v[in0, in0_valid, out0_ready, out1_ready])
     vec_to_streams' <| register_wrapper
       (inputs := vec_streams)
       (init_regs := #v[0#1, 0#1])
-      (update_fun := -- (Vector (BitVec 1) 7 × Vector (BitVec 1) 2) → (Vector α 9 × Vector α 2)
+      (update_fun :=
         fun (inp, regs) =>
           let v2 := BitVec.xor regs[0] 1#1
           let v3 := BitVec.and v2 inp[1]
-          let v4 := BitVec.and inp[4] v3
-          let v5 := BitVec.or v4 regs[0]
+          let v4 := BitVec.and inp[2] v3
+          let v5 := BitVec.or regs[0] v4
           let v8 := BitVec.xor regs[1] 1#1
           let v9 := BitVec.and v8 inp[1]
-          let v10 := BitVec.and inp[5] v9
+          let v10 := BitVec.and inp[3] v9
           let v11 := BitVec.or v10 regs[1]
           let v12 := BitVec.and v5 v11
-          let v6 := BitVec.xor v12 1#1
-          let v7 := BitVec.and v11 v6
           let v0 := BitVec.xor v12 1#1
           let v1 := BitVec.and v5 v0
           let updated_reg0 := v1
+          let v6 := BitVec.xor v12 1#1
+          let v7 := BitVec.and v11 v6
           let updated_reg1 := v7
-          (#v[v12, inp[6], 0#1, v3, 0#1, v9, inp[2], inp[3]], #v[updated_reg0, updated_reg1])
+          (#v[v12, inp[0], v3, inp[0], v9], #v[updated_reg0, updated_reg1])
       )
 
-/-- We prove that the description at handshake level and the description at lower (RTL) level are bisimilar. -/
-theorem fork_bisim
-    (arg0_data arg0_valid arg1_data arg1_valid out0_ready out1_ready out2_ready : Stream' (BitVec 1))
-    (arg0 arg1 out0 out1 out2 : Stream (BitVec 1)) :
-    let := ReadyValid #v[arg0_data, arg0_valid, arg0_ready] arg0
-    let := ReadyValid #v[arg1_data, arg1_valid, arg1_ready] arg1
-    let := ReadyValid #v[out0_data, out0_valid, out0_ready] out0
-    let := ReadyValid #v[out1_data, out1_valid, out1_ready] out1
-    let := ReadyValid #v[out2_data, out2_valid, out2_ready] out2
-    Bisim (iso_unary' ((fork_seq arg0_data arg0_valid arg1_data arg1_valid out0_ready oue1_ready out2_ready).get 0))  (fork_handshake arg0).fst := by
-  unfold iso_unary'
-  unfold Bisim
-  simp
+/--
+  The second configuration of the rtl-lowered program
 
-  sorry
+  hw.module @handshake_buffer_2slots_seq_1ins_1outs_ctrl(in %in0 : i0, in %in0_valid : i1, in %clock : !seq.clock, in %reset : i1, in %out0_ready : i1, out in0_ready : i1, out out0 : i0, out out0_valid : i1) {
+    %true = hw.constant true
+    %false = hw.constant false
+    %c0_i0 = hw.constant 0 : i0
+    %valid0_reg = seq.compreg sym @valid0_reg %2, %clock reset %reset, %false : i1
+    %0 = comb.xor %valid0_reg, %true : i1
+    %1 = comb.or %0, %5 : i1
+    %2 = comb.mux %1, %in0_valid, %valid0_reg : i1
+    %3 = comb.mux %1, %in0, %data0_reg : i0
+    %data0_reg = seq.compreg sym @data0_reg %3, %clock reset %reset, %c0_i0 : i0
+    %ready0_reg = seq.compreg sym @ready0_reg %10, %clock reset %reset, %false : i1
+    %4 = comb.mux %ready0_reg, %ready0_reg, %valid0_reg : i1
+    %5 = comb.xor %ready0_reg, %true : i1
+    %6 = comb.xor %15, %true : i1
+    %7 = comb.and %6, %5 : i1
+    %8 = comb.mux %7, %valid0_reg, %ready0_reg : i1
+    %9 = comb.and %15, %ready0_reg : i1
+    %10 = comb.mux %9, %false, %8 : i1
+    %ctrl_data0_reg = seq.compreg sym @ctrl_data0_reg %13, %clock reset %reset, %c0_i0 : i0
+    %11 = comb.mux %ready0_reg, %ctrl_data0_reg, %data0_reg : i0
+    %12 = comb.mux %7, %data0_reg, %ctrl_data0_reg : i0
+    %13 = comb.mux %9, %c0_i0, %12 : i0
+    %valid1_reg = seq.compreg sym @valid1_reg %16, %clock reset %reset, %false : i1
+    %14 = comb.xor %valid1_reg, %true : i1
+    %15 = comb.or %14, %19 : i1
+    %16 = comb.mux %15, %4, %valid1_reg : i1
+    %17 = comb.mux %15, %11, %data1_reg : i0
+    %data1_reg = seq.compreg sym @data1_reg %17, %clock reset %reset, %c0_i0 : i0
+    %ready1_reg = seq.compreg sym @ready1_reg %24, %clock reset %reset, %false : i1
+    %18 = comb.mux %ready1_reg, %ready1_reg, %valid1_reg : i1
+    %19 = comb.xor %ready1_reg, %true : i1
+    %20 = comb.xor %out0_ready, %true : i1
+    %21 = comb.and %20, %19 : i1
+    %22 = comb.mux %21, %valid1_reg, %ready1_reg : i1
+    %23 = comb.and %out0_ready, %ready1_reg : i1
+    %24 = comb.mux %23, %false, %22 : i1
+    %ctrl_data1_reg = seq.compreg sym @ctrl_data1_reg %27, %clock reset %reset, %c0_i0 : i0
+    %25 = comb.mux %ready1_reg, %ctrl_data1_reg, %data1_reg : i0
+    %26 = comb.mux %21, %data1_reg, %ctrl_data1_reg : i0
+    %27 = comb.mux %23, %c0_i0, %26 : i0
+    hw.output %1, %25, %18 : i1, i0, i1
+-/
+def handshake_buffer_2slots_seq_1ins_1outs_ctrl
+      (in0 : Stream' (BitVec 1))
+      (in0_valid : Stream' (BitVec 1))
+      (out0_ready : Stream' (BitVec 1))
+  : Vector (Stream' (BitVec 1)) 3 :=
+    let vec_streams := streams_to_vec'
+                        (#v[in0, in0_valid, out0_ready])
+    vec_to_streams' <| register_wrapper
+      (inputs := vec_streams) (r := 3)
+      (init_regs := #v[0#1, 0#1, 0#1, 0#1, 0#1, 0#1, 0#1, 0#1])
+      (update_fun :=
+        fun (inp, regs) =>
+          /- order of registers:
+            valid0, data0, ready0, ctrl_data0, valid1, data1, ready1, ctrl_data1 -/
+          let v5 := BitVec.xor regs[2] 1#1
+          let v14 := BitVec.xor regs[4] 1#1
+          let v19 := BitVec.xor regs[6] 1#1
+          let v15 := BitVec.or v14 v19
+          let v20 := BitVec.xor inp[2] 1#1
+          let v21 := BitVec.and v20 v19
+          let v22 := if v21.msb then regs[4] else regs[6]
+          let v23 := BitVec.and inp[2] regs[6]
+          let v24 := if v23.msb then 0#1 else v22
+          let v26 := if v21.msb then regs[5] else regs[7]
+          let v27 := if v23.msb then 0#1 else v26
+          let v0 := BitVec.xor regs[0] 1#1
+          let v1 := BitVec.or v0 v5
+          let v2 := if v1.msb then inp[1] else regs[0]
+          let v3 := if v1.msb then inp[0] else regs[1]
+          let v4 := if regs[2].msb then regs[2] else regs[0]
+          let v6 := BitVec.xor v15 1#1
+          let v7 := BitVec.and v5 v6
+          let v8 := if v7.msb then regs[0] else regs[2]
+          let v9 := BitVec.and v15 regs[2]
+          let v10 := if v9.msb then 0#1 else v8
+          let v11 := if regs[2].msb then regs[3] else regs[1]
+          let v12 := if v7.msb then regs[2] else regs[3]
+          let v13 := if v9.msb then 0#1 else v12
+          let v16 := if v15.msb then v4 else regs[4]
+          let v17 := if v15.msb then v11 else regs[5]
+          let v18 := if regs[6].msb then regs[6] else regs[4]
+          let v25 := if regs[6].msb then regs[7] else regs[5]
+          let updated_valid0 := v2
+          let updated_data0 := v3
+          let updated_ready0 := v10
+          let updated_ctrl_data0 := v13
+          let updated_valid1 := v16
+          let updated_data1 := v17
+          let updated_ready1 := v24
+          let updated_ctrl_data1 := v27
+          ⟨#v[v1, v25, v18], #v[updated_valid0, updated_data0, updated_ready0, updated_ctrl_data0,
+                                  updated_valid1, updated_data1, updated_ready1, updated_ctrl_data1]⟩
+      )
